pcuic/theories/PCUICNestedToMutual.v
@@ -9,6 +9,7 @@ From MetaRocq.PCUIC Require Import PCUICAst PCUICAstUtils PCUICOnFreeVars PCUICI
 From MetaRocq.PCUIC Require Import PCUICSigmaCalculus PCUICInstConv.
 Import PCUICEnvironment.
 From MetaRocq.PCUIC Require Import PCUICAuxToMove PCUICViewInductive.
+From MetaRocq.PCUIC Require Import BDStrengthening.
 Import ViewInductive.
 
 
@@ -18,6 +19,9 @@ Import ViewInductive.
     [X] 1.1 all but nested case
     [X] 1.2 nested case
     [ ] 1.3 indices
+      [X] change instantiation
+      [ ] filter indices
+      [ ] changes indices everywhere
 [ ] 2. Proof positivity is preserved
     [X] 2.1 all but nested case
     [X] 2.2 nested case
@@ -33,12 +37,183 @@ Indices :
 
 *)
 
+  Definition on_free_vars_andb P Q t :
+    on_free_vars P t && on_free_vars Q t = on_free_vars (fun x => P x && Q x) t.
+  Proof.
+  Admitted.
+
+  Definition on_free_vars_impl2 {q1 q2 p : nat -> bool} {t} :
+    (forall i, q1 i -> q2 i -> p i) ->
+    on_free_vars q1 t -> on_free_vars q2 t ->  on_free_vars p t.
+  Proof.
+    intros H Hq1 Hq2. eapply on_free_vars_impl with (p := fun i => q1 i && q2 i).
+    1: { intros i [? ?]%andb_prop. apply H => //. }
+    rewrite -on_free_vars_andb. apply andb_true_intro. by constructor.
+  Qed.
+
+(* check if the var is in *)
+  Definition on_free_var_of_rev_list (l : list bool) k : term -> bool :=
+    on_free_vars (shiftnP k (fun n => ~~ (nth n (List.rev l) false))).
+
+  Definition All_sym_inv : forall {A B C : Type} (f : A -> C) (g : B -> C)
+    l l',
+    All2 (fun y x => f x = g y) l' l ->
+    All2 (fun x y => f x = g y) l  l'.
+  Proof.
+    intros * X; induction X; constructor; eauto.
+  Qed.
+
+
+
+
+
+  (* Strengthening *)
+  Axiom (rename_argument : forall (f : nat -> nat) (above : nat), argument -> argument).
+
+  (* Definition rename (f : nat -> nat) (above : nat) : term -> term :=
+    rename (shiftn above f). *)
+
+  Definition strengthen_renaming k f : nat -> nat :=
+    fun n => if n <? k then n else f (n - k).
+
+  Definition strengthen_term k : term -> term :=
+    rename (strengthen_renaming k (fun n => n)).
+
+  Definition strengthen_pred k P : nat -> bool :=
+    fun n => P (n + k).
+
+  Definition on_free_vars_strengthen P k t :
+    on_free_vars (fun n => k-1 <? n) t ->
+    on_free_vars P t ->
+    on_free_vars (strengthen_pred k P) (strengthen_term k t).
+  Proof.
+    intros Hnotin Ht.
+    assert (Hboth : on_free_vars (fun n => P n && (k - 1 <? n)) t).
+      1: { rewrite -on_free_vars_andb. apply andb_true_intro. constructor => //. }
+    rewrite on_free_vars_rename. eapply on_free_vars_impl; only 2 : exact Hboth; cbn.
+    unfold strengthen_pred, strengthen_renaming.
+    intros i. intros [Pi ki]%andb_prop.
+    assert (i <? k = false) as -> by lia.
+    replace (i - k + k) with i by lia; done.
+  Qed.
+
+  Definition on_free_vars_shiftn_strengthen P k t :
+    on_free_vars (fun n => k-1 <? n) t ->
+    on_free_vars (shiftnP k P) t ->
+    on_free_vars P (strengthen_term k t).
+  Proof.
+    intros Hnotin Ht.
+    rewrite on_free_vars_rename.
+    refine (on_free_vars_impl2 _ Hnotin Ht).
+    unfold shiftnP, strengthen_renaming.
+    intros i ki [ik | Pik]%orb_prop; hnf in ki; try lia.
+    assert (i <? k = false) as -> by lia.
+    replace (i - k + k) with i by lia; done.
+  Qed.
+
+  Axiom (strengthen_argument : nat -> argument -> argument).
+  Axiom (on_free_vars_argument : (nat -> bool) -> argument -> bool).
+
+  Section StrengthArg.
+    Context (nb_block : nat).
+    Context (up : list (context_decl * bool)).
+    Context (nup : context).
+
+  Definition strengthen_k_pos Γ Δ lax nb_binders arg k :
+    on_free_vars_argument (fun n => k -1 <? n) arg ->
+    positive_argument nb_block up nup (Γ ++ Δ) lax nb_binders arg ->
+    positive_argument nb_block up nup Γ lax nb_binders (strengthen_argument #|Δ| arg).
+  Proof.
+  Admitted.
+
+
+
+  (* remove one arg or update it, and the renaming function  *)
+  Definition remove_rc_one (acc : list argument * (nat -> nat)) (arg : argument )
+      : list argument * (nat -> nat) :=
+    if check_lax arg
+    then (acc.1, strengthen_renaming 1 acc.2)
+    else (acc.1 ++ [rename_argument acc.2 0 arg], shiftn 1 acc.2).
+
+  (* What would be the spec ??? *)
+
+
+
+
+  Definition remove_rc_args Γ : list argument :=
+    (fold_left remove_rc_one Γ ([],fun n => n)).1.
+
+  Definition remove_rc_rename Γ : nat -> nat :=
+    (fold_left remove_rc_one Γ ([],fun n => n)).2.
+
+  Fixpoint comp_offset (l : list bool) acc : list nat :=
+      match l with
+      | [] => []
+      | true::l => acc :: comp_offset l (acc + 1)
+      | false::l => acc :: comp_offset l acc
+      end.
+
+  (* properties *)
+  Definition pos_remove_rc (Γ : list argument) (t : term) :
+    ind_sp_uparams_notin up #|Γ| t ->
+    on_free_var_of_rev_list (map check_lax Γ) 0 t ->
+    ind_sp_uparams_notin up #|remove_rc_args Γ|
+        (rename (remove_rc_rename Γ) t).
+  Proof.
+  Admitted.
+
+  Definition length_remove_rec_call Γ acc :
+    #|filter (fun t => ~~ check_lax t) Γ| + #|acc.1| =
+    #|(fold_left remove_rc_one Γ acc).1|.
+  Proof.
+    clear. revert acc.
+    unfold remove_rc_one.
+    induction Γ as [|a Γ IHΓ]; cbn => //.
+    intros [args f]. destruct (check_lax a); cbn.
+    rewrite -IHΓ; cbn; cbn_length; cbn. reflexivity.
+    rewrite -IHΓ; cbn; cbn_length; cbn. lia.
+  Qed.
+
+End StrengthArg.
+
+
+(* Tests
+
+  Definition try1 := [false; false; true; false; true; true; false].
+
+  Definition cpt_args2 (acc : list bool * (nat -> nat)) (b : bool)
+      : list bool * (nat -> nat) :=
+    if b
+    then (acc.1, strengthen 1 acc.2)
+    else (acc.1 ++ [b], shiftn 1 acc.2).
+
+  Definition ff2 : nat -> nat
+    := (fold_left cpt_args2 try1 ([],fun n => n)).2.
+
+  (*
+  -------------------------------------
+  | 8 | 7 | 6 | 5 | 4 | 3 | 2 | 1 | 0 |
+  -------------------------------------
+  | 5 | 4 | 3 | 2 | X | 1 | X | X | 0 |
+  -------------------------------------
+  *)
+
+  Compute (ff2 8). Compute (ff2 7). Compute (ff2 6). Compute (ff2 5).
+  Compute (ff2 4). Compute (ff2 3). Compute (ff2 2). Compute (ff2 1).
+  Compute (ff2 0).
+*)
+
+
+  Definition rename (f : nat -> nat) (above : nat) : term -> term :=
+    rename (shiftn above f).
 
 (* *** Nested to Mutual *** *)
 
 Section NestedToMutualInd.
 
-  (*** Information Global Inductive Type ***)
+  (* 1. ### Info Nesting ### *)
+
+  (* Information Global Inductive Type *)
   Context (nb_g_block : nat).
 
   Context (g_uparams_b  : list (context_decl * bool)).
@@ -49,55 +224,33 @@ Section NestedToMutualInd.
   Notation nb_g_nuparams := #|g_nuparams|.
 
   (* Context of the nesting *)
-    (* arguments already seen *)
-    Context (g_Γargs : list argument).
-    Notation nb_g_args := #|g_Γargs|.
+  (* arguments already seen *)
+  Context (g_args : list argument).
+  Notation nb_g_args := #|g_args|.
+  Context (pos_g_args : All_telescope (fun Γ => positive_argument nb_g_block g_uparams_b g_nuparams (map check_lax Γ) true 0) g_args).
 
-    Definition g_args : context :=
-      arguments_to_context nb_g_block g_uparams_b (nb_g_uparams + nb_g_nuparams) g_Γargs.
+  (* Argument to the left of nesting  *)
+  Context (g_largs : list term).
+  Notation nb_g_largs := #|g_largs|.
 
-    Context (pos_g_Γargs : All_telescope (fun Γargs => positive_argument nb_g_block g_uparams_b g_nuparams (map check_lax Γargs) true 0) g_Γargs).
+  Context (pos_g_largs : Alli (ind_sp_uparams_notin g_uparams_b) (nb_g_nuparams + nb_g_args) g_largs).
 
-    (* Argument to the left of nesting  *)
-    Context (g_largs_t : list term).
-    Notation nb_g_largs := #|g_largs_t|.
-
-    Definition g_largs : context := cxt_of_terms (g_largs_t).
-
-    Context (pos_g_largs_t : Alli (ind_sp_uparams_notin g_uparams_b) (nb_g_nuparams + nb_g_args) g_largs_t).
-
-
-  (*** Information about the inductive type used for nesting ***)
+  (* Information about the inductive type used for nesting *)
   Context (nb_l_block : nat).
-
-  (* total block *)
   Notation nb_m_block := (nb_g_block + nb_l_block).
 
-  (* uparams *)
   Context (l_uparams_b : list (context_decl * bool)).
   Notation nb_l_uparams  := #|l_uparams_b|.
 
-  Definition l_uparams : context := map fst l_uparams_b.
-
-  (* nuparams *)
   Context (l_nuparams : context).
   Notation nb_l_nuparams := #|l_nuparams|.
-
-  (* Definition l_nuparams_t : list term := terms_of_cxt l_nuparams. *)
-
   Context (pos_l_nuparams : Alli (ind_sp_uparams_notin l_uparams_b) 0
-                                 (terms_of_cxt l_nuparams)).
+                                (terms_of_cxt l_nuparams)).
 
-  (* parameters *)
-  (* Definition l_params : context := l_uparams ,,, l_nuparams.
-  Notation nb_l_params := (nb_l_uparams + nb_l_nuparams). *)
-
-
-  (* instantiation turn to a list of terms *)
-  Notation nb_cxt_sub := (nb_g_nuparams + nb_g_args + nb_g_largs).
+  (* Instantiation Nesting *)
+  Notation nb_old_cxt_sub := (nb_g_nuparams + nb_g_args + nb_g_largs).
 
   Context (inst_uparams_a : list (list term * argument)).
-
   Context (spec_inst_uparams_a :
       All2 (fun x y  =>
           let llargs := x.1 in let arg := x.2 in
@@ -105,46 +258,43 @@ Section NestedToMutualInd.
         (* fully applied ensured by typing*)
           (#|llargs| = cdecl_to_arity cdecl)
           (* llargs are free *)
-        * Alli (ind_sp_uparams_notin g_uparams_b) nb_cxt_sub llargs
+        * Alli (ind_sp_uparams_notin g_uparams_b) nb_old_cxt_sub llargs
           (* args are pos lax or strict depending if you can nest or not *)
-        * positive_argument nb_g_block g_uparams_b g_nuparams (map check_lax g_Γargs) pos (nb_g_largs + #|llargs|) arg
-    ) inst_uparams_a (rev l_uparams_b)).
+        * positive_argument nb_g_block g_uparams_b g_nuparams (map check_lax g_args) pos (nb_g_largs + #|llargs|) arg
+    ) inst_uparams_a (List.rev l_uparams_b)).
 
+
+  (* ### 2. Old Spec ### *)
   Definition size_inst_uparams : #|inst_uparams_a| = nb_l_uparams.
   Proof.
-    rewrite -(length_rev (l := l_uparams_b)).
+    cbn_length.
+    rewrite -(List.length_rev (l_uparams_b)).
     eapply All2_length; tea.
   Qed.
 
-  Definition All_sym_inv : forall {A B C : Type} (f : A -> C) (g : B -> C)
-    l l',
-    All2 (fun y x => f x = g y) l' l ->
-    All2 (fun x y => f x = g y) l  l'.
+  (* !!! rev to remove at a point => probably keep reversing eq *)
+  Definition fapp_inst_uparams_a : All2 (fun n x => n = #|x.1|)
+      (List.rev (uparams_nb_args l_uparams_b)) inst_uparams_a.
   Proof.
-    intros * X; induction X; constructor; eauto.
-  Qed.
-
-  Definition fapp_inst_uparams : All2 (fun n x => n = #|x.1|)
-      (rev (uparams_nb_args l_uparams_b)) inst_uparams_a.
-  Proof.
-    rewrite -map_rev -(map_id inst_uparams_a).
+    rewrite -List.map_rev -(map_id inst_uparams_a).
     eapply All2_map. eapply All_sym_inv.
     eapply All2_impl; only 1 : apply spec_inst_uparams_a.
     intros [llargs arg] [cdecl pos]; cbn.
-    intros []; now symmetry.
+    intros [[]]; solve_length.
   Qed.
 
-  (* awfull !!! *)
   Definition positive_inst_llargs :
-    All (fun p => Alli (ind_sp_uparams_notin g_uparams_b) nb_cxt_sub p.1) inst_uparams_a.
+    All (fun p => Alli (ind_sp_uparams_notin g_uparams_b) nb_old_cxt_sub p.1)
+        inst_uparams_a.
   Proof.
-    induction spec_inst_uparams_a; cbn in spec_inst_uparams_a; constructor. inversion spec_inst_uparams_a. subst.
-    destruct x, y; cbn in *. destruct r as [ []]. assumption.
+    induction spec_inst_uparams_a; cbn in spec_inst_uparams_a; constructor.
+    inversion spec_inst_uparams_a. subst.
+    destruct x as [llargs arg], y as [cdecl pos], r as [[fapp pos_llargs] pos_arg]; cbn in * => //.
     apply IHa. assumption.
   Qed.
 
   Definition positive_true_all :
-    All (fun x => positive_argument nb_g_block g_uparams_b g_nuparams (map check_lax g_Γargs)
+    All (fun x => positive_argument nb_g_block g_uparams_b g_nuparams (map check_lax g_args)
                       true (nb_g_largs + #|x.1|) x.2) inst_uparams_a.
   Proof.
     induction spec_inst_uparams_a; constructor; cbn; eauto.
@@ -152,50 +302,194 @@ Section NestedToMutualInd.
     destruct pos => //. apply pos_argument_from_false => //.
   Qed.
 
+  Definition inst_to_term_old : (list term * argument) -> term :=
+  fun '(llargs, arg) =>
+    (it_tLambda llargs (argument_to_term nb_g_block g_uparams_b (nb_old_cxt_sub + #|llargs|) arg)).
 
-  Definition inst_to_term : (list term * argument) -> term :=
-    fun '(llargs, arg) => it_tLambda llargs (argument_to_term nb_g_block g_uparams_b (nb_cxt_sub + #|llargs|) arg).
-
-  Definition pos_inst_to_term :
-    All2 (fun ' (llargs, arg) ' (cdecl, pos) =>
-        pos = false -> ind_sp_uparams_notin g_uparams_b (nb_cxt_sub) (inst_to_term (llargs, arg))
-    ) inst_uparams_a (rev l_uparams_b).
+  Definition pos_inst_to_term_old :
+    All2 (fun x y =>
+        y.2 = false -> ind_sp_uparams_notin g_uparams_b (nb_old_cxt_sub) (inst_to_term_old x)
+    ) inst_uparams_a (List.rev l_uparams_b).
   Proof.
     eapply All2_impl ; [exact spec_inst_uparams_a|].
     intros [llargs arg] [cdecl pos] [[fapp_llargs notin_llargs] pos_arg]; cbn in *.
     destruct pos. 1: intros x; inversion x.
-    intros _. unfold inst_to_term.
+    intros _. unfold inst_to_term_old.
     apply ind_sp_uparams_notin_tLambda => //.
     destruct (positive_argument_strict _ _ _ _ pos_arg) as [t ->]; cbn.
     inversion pos_arg => //. eapply eq_notin; only 2: tea; solve_length.
   Qed.
 
+
+  (* 3. ### New args context and subsitution and properties ### *)
+
+  Definition rc_notin : nat -> term -> bool
+    := on_free_var_of_rev_list (map check_lax g_args).
+
+  Definition rc_notin_args : nat -> argument -> bool :=
+    todo.
+
+  Axiom (notin_g_largs : Alli rc_notin 0 g_largs).
+  Axiom (notin_inst_llargs_args :
+    All (fun p => Alli rc_notin nb_g_largs p.1
+                  * rc_notin_args (nb_g_largs + #|p.1|) p.2)
+    inst_uparams_a).
+
+
+  (* New args + Spec *)
+  Definition g_args_no_rc : list argument :=
+    (fold_left remove_rc_one g_args ([],fun n => n)).1.
+
+  Definition pos_g_args_no_rc :
+    All_telescope (fun Γ => positive_argument nb_g_block g_uparams_b g_nuparams
+      (map check_lax Γ) true 0) g_args_no_rc.
+  Admitted.
+
+  (* New renaming + Spec *)
+  Definition rename_no_rc : nat -> nat :=
+    (fold_left remove_rc_one g_args ([],fun n => n)).2.
+
+  Definition length_g_args_no_rc :
+    #|filter (fun t => ~~ check_lax t) g_args| = #|g_args_no_rc|.
+  Proof.
+    rewrite -length_remove_rec_call //= Nat.add_0_r.
+  Qed.
+
+  Notation nb_g_args_no_rc := (#|g_args_no_rc|).
+  Notation nb_new_cxt_sub := (nb_g_nuparams + nb_g_args_no_rc + nb_g_largs).
+
+  Definition pos_rename_no_rc i t :
+    rc_notin i t ->
+    ind_sp_uparams_notin g_uparams_b (nb_g_nuparams + nb_g_args + i) t ->
+    ind_sp_uparams_notin g_uparams_b (nb_g_nuparams + nb_g_args_no_rc + i)
+                                      (rename rename_no_rc i t).
+  Proof.
+  Admitted.
+
+  Definition pos_rename_no_rc_arg lax i arg :
+    rc_notin_args i arg ->
+    positive_argument nb_g_block g_uparams_b g_nuparams (map check_lax g_args) lax i arg ->
+    positive_argument nb_g_block g_uparams_b g_nuparams (map check_lax g_args_no_rc) lax i
+                                      (rename_argument rename_no_rc i arg).
+  Proof.
+  Admitted.
+
+
+  (* 4. Update instantiation and properties *)
+  Definition g_largs_no_rc : list term :=
+    mapi (rename rename_no_rc) g_largs.
+
+  Definition pos_g_largs_no_rc :
+    Alli (ind_sp_uparams_notin g_uparams_b) (nb_g_nuparams + nb_g_args_no_rc) g_largs_no_rc.
+  Proof.
+    refine (Alli_mapi2 _ notin_g_largs pos_g_largs); cbn.
+    apply pos_rename_no_rc.
+  Qed.
+
+  Definition inst_uparams_no_rc : list (list term * argument) :=
+    map (fun ' (llargs, arg) =>
+      let llargs' := mapi (fun i => rename rename_no_rc (nb_g_largs + i)) llargs in
+      let arg' := rename_argument rename_no_rc (nb_g_largs + #|llargs|) arg in
+      (llargs', arg')
+      )
+    inst_uparams_a.
+
+  Definition size_inst_uparams_no_rc : #|inst_uparams_no_rc| = nb_l_uparams.
+  Proof.
+    cbn_length. rewrite -(List.length_rev (l_uparams_b)). eapply All2_length; tea.
+  Qed.
+
+  Definition fapp_inst_uparams_no_rc : All2 (fun n x => n = #|x.1|)
+      (List.rev (uparams_nb_args l_uparams_b)) inst_uparams_no_rc.
+  Proof.
+    rewrite -List.map_rev -(map_id inst_uparams_no_rc).
+    eapply All2_map. eapply All_sym_inv.
+    apply All2_map_left.
+    eapply All2_impl; only 1 : apply spec_inst_uparams_a.
+    intros [llargs arg] [cdecl pos]; cbn.
+    intros [[]]; solve_length.
+  Qed.
+
+  Definition positive_inst_llargs_no_rc :
+    All (fun p => Alli (ind_sp_uparams_notin g_uparams_b) nb_new_cxt_sub p.1)
+        inst_uparams_no_rc.
+  Proof.
+    unfold inst_uparams_no_rc.
+    refine (All_map2 _ positive_inst_llargs notin_inst_llargs_args).
+    intros [llargs arg]; cbn. intros X [Y _].
+    refine (Alli_mapi2 _ X Y).
+    intros. eapply eq_notin.
+    2: { apply pos_rename_no_rc => //. eapply eq_notin; tea. lia. }
+    lia.
+  Qed.
+
+  Definition positive_true_all_no_rc :
+    All (fun x => positive_argument nb_g_block g_uparams_b g_nuparams (map check_lax g_args_no_rc)
+                      true (nb_g_largs + #|x.1|) x.2) inst_uparams_no_rc.
+  Proof.
+    unfold inst_uparams_no_rc.
+    refine (All_map2 _ notin_inst_llargs_args positive_true_all).
+    intros [llargs arg]; cbn_length; cbn. intros [_ ?] ?.
+    apply pos_rename_no_rc_arg => //.
+  Qed.
+
+  (* 5. instantiation *)
+
+  (* should not have renaming as applied to inst_uparams_no_rc *)
+  Definition inst_to_term : (list term * argument) -> term :=
+    fun '(llargs, arg) =>
+      (it_tLambda llargs (argument_to_term nb_g_block g_uparams_b (nb_new_cxt_sub + #|llargs|) arg)).
+
+  Axiom (rename_argument_free : forall a b c f k t, argument_to_term a b c (rename_argument f k (arg_is_free t)) = rename f k t).
+
+  Definition pos_inst_to_term :
+    All2 (fun x y =>
+        y.2 = false -> ind_sp_uparams_notin g_uparams_b (nb_new_cxt_sub) (inst_to_term x)
+    ) inst_uparams_no_rc (List.rev l_uparams_b).
+  Proof.
+    unfold inst_uparams_no_rc.
+    eapply All2_map_left. eapply All2_impl2.
+    + apply spec_inst_uparams_a.
+    + apply All2_left_triv. 2: rewrite size_inst_uparams; solve_length. apply notin_inst_llargs_args.
+    + intros [llargs arg] [cdecl pos] [[fapp_llargs notin_llargs] pos_arg]
+        [notin_llarg notin_arg] pos_lax. cbn in *. cbn_length.
+      apply ind_sp_uparams_notin_tLambda => //.
+      - refine (Alli_mapi2 _ notin_llarg notin_llargs); cbn. intros.
+        eapply eq_notin; only 2: apply pos_rename_no_rc => //. lia.
+        eapply eq_notin; tea; solve_length.
+      - rewrite pos_lax in pos_arg.
+        destruct (positive_argument_strict _ _ _ _ pos_arg) as [t ->]; cbn.
+        rewrite rename_argument_free. cbn_length.
+        eapply eq_notin; only 2: apply pos_rename_no_rc.
+      * lia.
+      * admit. (* ok *)
+      * admit. (* ok *)
+  Admitted.
+
   Definition inst_uparams : nat -> term :=
-    fun n => nth n (map inst_to_term inst_uparams_a) (tRel n).
+    fun n => nth n (map inst_to_term inst_uparams_no_rc) (tRel n).
 
   (* check that if n uparams is not positive
      then the instantiation does not contain the variable
   *)
   Definition pos_inst_uparams : forall n,
     ind_sp_uparams_notinP l_uparams_b n ->
-    ind_sp_uparams_notin g_uparams_b nb_cxt_sub (inst_uparams n).
+    ind_sp_uparams_notin g_uparams_b nb_new_cxt_sub (inst_uparams n).
   Proof.
     intros n. unfold ind_sp_uparams_notinP, andP, ind_notinP, sp_uparams_notinP.
     intros x%andb_prop; destruct x as [notInd notSpUparams].
     destruct (Nat.lt_ge_cases n nb_l_uparams) as [nleb | nlt].
     - unfold inst_uparams.
       rewrite negb_true_iff in notSpUparams. revert notSpUparams.
-      apply (All2_nth (fun x y => y.2 = false -> ind_sp_uparams_notin g_uparams_b nb_cxt_sub x)).
+      apply (All2_nth (fun x y => y.2 = false -> ind_sp_uparams_notin g_uparams_b nb_new_cxt_sub x)).
       1: cbn_length; rewrite size_inst_uparams //.
-      rewrite -(map_id (rev l_uparams_b)).
-      apply All2_map. eapply All2_impl. 1: apply pos_inst_to_term.
-      now intros [] [].
+      apply All2_map_left. apply pos_inst_to_term.
     - apply leb_correct in nlt. rewrite nlt in notInd. inversion notInd.
   Qed.
 
   Definition inst_preserve_not (k : nat) t :
     ind_sp_uparams_notin l_uparams_b k t ->
-    ind_sp_uparams_notin g_uparams_b (nb_cxt_sub + k) t.[up k inst_uparams].
+    ind_sp_uparams_notin g_uparams_b (nb_new_cxt_sub + k) t.[up k inst_uparams].
   Proof.
     rewrite Nat.add_comm. apply on_free_vars_inst.
     intros n. rewrite <- shiftnP_add. apply on_free_vars_up.
@@ -203,7 +497,7 @@ Section NestedToMutualInd.
   Qed.
 
   Definition inst_preserve_not_eq (k m : nat) t :
-    m = nb_cxt_sub + k ->
+    m = nb_new_cxt_sub + k ->
     ind_sp_uparams_notin l_uparams_b k t ->
     ind_sp_uparams_notin g_uparams_b m t.[up k inst_uparams].
   Proof.
@@ -212,14 +506,14 @@ Section NestedToMutualInd.
 
   Definition All_notin k l :
     All (ind_sp_uparams_notin l_uparams_b k) l ->
-    All (ind_sp_uparams_notin g_uparams_b (nb_cxt_sub + k))
+    All (ind_sp_uparams_notin g_uparams_b (nb_new_cxt_sub + k))
             (map (fun t => t.[up k inst_uparams]) l).
   Proof.
     apply All_map. apply inst_preserve_not.
   Qed.
 
   Definition All_notin_eq k m l :
-  m = nb_cxt_sub + k ->
+  m = nb_new_cxt_sub + k ->
   All (ind_sp_uparams_notin l_uparams_b k) l ->
   All (ind_sp_uparams_notin g_uparams_b m) (map (fun t => t.[up k inst_uparams]) l).
   Proof.
@@ -228,7 +522,7 @@ Section NestedToMutualInd.
 
   Definition Alli_notin l k :
   Alli (ind_sp_uparams_notin l_uparams_b) k l ->
-  Alli (ind_sp_uparams_notin g_uparams_b) (nb_cxt_sub + k)
+  Alli (ind_sp_uparams_notin g_uparams_b) (nb_new_cxt_sub + k)
           (mapi_rec (fun i t => t.[up i inst_uparams]) l k).
   Proof.
     rewrite Nat.add_comm.
@@ -237,7 +531,7 @@ Section NestedToMutualInd.
   Qed.
 
   Definition Alli_notin_eq l k m :
-  m = (nb_cxt_sub + k) ->
+  m = (nb_new_cxt_sub + k) ->
   Alli (ind_sp_uparams_notin l_uparams_b) k l ->
   Alli (ind_sp_uparams_notin g_uparams_b) m
           (mapi_rec (fun i t => t.[up i inst_uparams]) l k).
@@ -282,11 +576,11 @@ Section NestedToMutualInd.
   forall (t : term),
   All (ind_sp_uparams_notin up k) s ->
   ind_sp_uparams_notin up (k + i + #|s|) t ->
-  ind_sp_uparams_notin up (k + i) (subst (rev s) i t).
+  ind_sp_uparams_notin up (k + i) (subst (List.rev s) i t).
   Proof.
     intros. apply ind_sp_uparams_notin_subst => //.
     - apply All_rev => //.
-    - now rewrite length_rev.
+    - now rewrite List.length_rev.
   Qed.
 
   Definition ind_sp_uparams_notin_subst_rev_eq up k i s m n :
@@ -295,7 +589,7 @@ Section NestedToMutualInd.
     n = k + i ->
     All (ind_sp_uparams_notin up k) s ->
     ind_sp_uparams_notin up m t ->
-    ind_sp_uparams_notin up n (subst (rev s) i t).
+    ind_sp_uparams_notin up n (subst (List.rev s) i t).
   Proof.
     intros t -> ->; apply ind_sp_uparams_notin_subst_rev.
   Qed.
@@ -321,22 +615,28 @@ Section NestedToMutualInd.
 
         g_args ,,, g_largs ,,,  σ(l_nuparams ,,, indices)
 
-    WARNING => this creates inductive-inductive types!
+    ISSUE => this creates inductive-inductive types!
             => it SHOULD be possible to be finer only add the context really
                needed and stay mutual
 
-      Sol1?: Make it so you only need the strict pos arg
-        V1:
-        => str pos can't be used in the rest of the context (needed anyway)
-        => a polymorphic argument ?
-        V2
-        => add by hand it in the pos condition, should work but v1 would be better
+    Solution: Remove rec call, i.e. strengthen including subst
 
-    This also forces us to add g_args ,,, g_largs ,,,  σ(l_nuparams) as
-    arguments of the constructors so that they can be refered in indices.
+      ↓↓g_args ,,, ↓g_largs ,,,  (↓σ)(l_nuparams ,,, indices)
 
-    Note 1 : Fundamentally g_args ,,, g_largs ,,,  σ(l_nuparams) are uparams
-    they are indices only because this must be common to all blocks.
+      Either:
+        V1: str pos can't be used in the rest of the context (needed anyway) + a polymorphic argument ?
+        V2: add by hand it in the pos condition, should work but v1 would be better
+
+      V1 should be true but hard to prove => This uses V2.
+
+    This also forces us to add:
+
+      ↓↓g_args ,,, ↓g_largs ,,,  (↓σ)(l_nuparams)
+
+    as arguments of the constructors so that they can be refered in indices.
+
+    Note 1 : Fundamentally they are are non uniform parameters,
+    they are indices only because parameters must be common to all blocks.
     That would be nice tough, as we wouldn't have to add them everywhere.
 
     Note 2 : We can not subtitute the intanciation of non-uniform pamareters nor
@@ -346,46 +646,47 @@ Section NestedToMutualInd.
 
   *)
 
-  (* TO BE FIXED LATED => how not to be ind-ind ?
-     Just filter out g_args that are not free ? *)
   Definition new_indices indices : context :=
-    g_args ,,, g_largs ,,, inst_context inst_uparams (l_nuparams ,,, indices).
+    arguments_to_context nb_g_block g_uparams_b (nb_g_uparams + nb_g_nuparams) g_args_no_rc ,,,
+    cxt_of_terms g_largs_no_rc ,,,
+    inst_context inst_uparams (l_nuparams ,,, indices).
 
 
   (* New Arguments + Positivity *)
   Definition cstr_new_args : list argument :=
-       g_Γargs
-    ++ map arg_is_free g_largs_t
+       g_args_no_rc
+    ++ map arg_is_free g_largs_no_rc
     ++ map arg_is_free (mapi_rec (fun i t => t.[up i inst_uparams])
         (terms_of_cxt l_nuparams) 0).
 
   Notation nb_new_args := #|cstr_new_args|.
 
-  Definition nb_new_args_unfold : nb_new_args = nb_g_args + nb_g_largs + nb_l_nuparams.
+  Definition nb_new_args_unfold : nb_new_args = nb_g_args_no_rc + nb_g_largs + nb_l_nuparams.
   Proof.
     solve_length.
   Qed.
 
 
   Definition pos_cstr_new_args :
-    All_telescope (fun Γargs => positive_argument nb_m_block g_uparams_b g_nuparams (map check_lax Γargs) true 0) cstr_new_args.
+    All_telescope (fun Γ => positive_argument nb_m_block g_uparams_b g_nuparams (map check_lax Γ) true 0) cstr_new_args.
   Proof.
     eapply All_telescope_impl; only 2: (intros ? ? X; apply pos_arg_inc; exact X).
     unfold cstr_new_args.
     repeat apply All_telescope_app_inv; cbn.
-    + assumption.
+    + apply pos_g_args_no_rc.
     + eapply All_telescope_map.
       - intros ? ? X; apply pos_arg_is_free. cbn_length. exact X.
       - apply All_telescope_to_Alli with
               (P := (fun n (x : term) => ind_sp_uparams_notin g_uparams_b n x))
-              (n := nb_g_nuparams + nb_g_args) => //.
+              (n := nb_g_nuparams + nb_g_args_no_rc) => //.
+        apply pos_g_largs_no_rc.
     + eapply All_telescope_map.
       - intros ? ? X; apply pos_arg_is_free; cbn_length; exact X.
       - apply All_telescope_to_Alli with
               (P := (fun n (x : term) => ind_sp_uparams_notin g_uparams_b (n) x))
-              (n := nb_cxt_sub).
+              (n := nb_new_cxt_sub).
         eapply Alli_mapi; tea. cbn. intros. apply inst_preserve_not_eq => //.
-  Defined.
+  Qed.
 
   (* Specialization of Arguments *)
 
@@ -398,22 +699,22 @@ Section NestedToMutualInd.
     match arg with
     | arg_is_free t => arg_is_free (it_tProd largs (mkApps (it_tLambda llargs t) args))
     | arg_is_sp_uparam ll k x =>
-        let ll' := mapi (fun i => subst (rev args) i) ll in
-        let x' := map (subst (rev args) #|ll|) x in
+        let ll' := mapi (fun i => subst (List.rev args) i) ll in
+        let x' := map (subst (List.rev args) #|ll|) x in
         arg_is_sp_uparam (largs ++ ll') k x'
     | arg_is_ind ll pos_indb i_upi =>
-        let ll' := mapi (fun i => subst (rev args) i) ll in
-        let i_upi' := map (subst (rev args) #|ll|) i_upi in
+        let ll' := mapi (fun i => subst (List.rev args) i) ll in
+        let i_upi' := map (subst (List.rev args) #|ll|) i_upi in
         arg_is_ind (largs ++ ll') pos_indb i_upi'
     | arg_is_nested ll ind u inst_up inst_else =>
-        let ll' := mapi (fun i => subst (rev args) i) ll in
+        let ll' := mapi (fun i => subst (List.rev args) i) ll in
         let inst_up'  := map (fun ' (llargs, arg) =>
-            let llargs' := mapi (fun i => subst (rev args) (#|ll| + i)) llargs in
-            let arg' := subst_argument (rev args) (#|ll| + #|llargs|) arg in
+            let llargs' := mapi (fun i => subst (List.rev args) (#|ll| + i)) llargs in
+            let arg' := subst_argument (List.rev args) (#|ll| + #|llargs|) arg in
             (llargs', arg')
             ) inst_up
           in
-        let inst_else' := map (subst (rev args) #|ll|) inst_else in
+        let inst_else' := map (subst (List.rev args) #|ll|) inst_else in
         arg_is_nested (largs ++ ll') ind u inst_up' inst_else'
     end.
 
@@ -426,17 +727,17 @@ Section NestedToMutualInd.
     ( eapply All_map; only 2: eassumption;
       intros x; eapply ind_sp_uparams_notin_subst_rev_eq; tea; lia).
 
-  Definition pos_sub_uparams Γargs largs args (lax : bool) nb_binders (llargs : list term) (arg : argument)
+  Definition pos_sub_uparams Γ largs args (lax : bool) nb_binders (llargs : list term) (arg : argument)
     (* contet substitution *)
-    (pos_largs : Alli (ind_sp_uparams_notin g_uparams_b) (nb_g_nuparams + #|Γargs| + nb_binders) largs)
-    (pos_args  : All  (ind_sp_uparams_notin g_uparams_b  (nb_g_nuparams + #|Γargs| + nb_binders + #|largs|)) args)
+    (pos_largs : Alli (ind_sp_uparams_notin g_uparams_b) (nb_g_nuparams + #|Γ| + nb_binders) largs)
+    (pos_args  : All  (ind_sp_uparams_notin g_uparams_b  (nb_g_nuparams + #|Γ| + nb_binders + #|largs|)) args)
     (* arg to substitute by *)
     (fapp_arg : #|llargs| = #|args|)
-    (pos_llargs : Alli (ind_sp_uparams_notin g_uparams_b) (nb_g_nuparams + #|Γargs| + nb_binders + #|largs|) llargs)
-    (pos_arg : positive_argument nb_m_block g_uparams_b g_nuparams Γargs
+    (pos_llargs : Alli (ind_sp_uparams_notin g_uparams_b) (nb_g_nuparams + #|Γ| + nb_binders + #|largs|) llargs)
+    (pos_arg : positive_argument nb_m_block g_uparams_b g_nuparams Γ
                   lax (nb_binders + #|largs| + #|llargs|) arg)
     :
-    positive_argument nb_m_block g_uparams_b g_nuparams Γargs
+    positive_argument nb_m_block g_uparams_b g_nuparams Γ
       lax nb_binders (sub_uparam largs args llargs arg).
   Proof.
     remember (nb_binders + #|largs| + #|llargs|) as p eqn:Heqp.
@@ -476,15 +777,14 @@ Section NestedToMutualInd.
         let largs' := mapi_rec (fun i t => t.[up i inst_uparams]) largs pos_sub_cxt in
         let args'  := map (fun t => t.[up (pos_sub_cxt + #|largs|) inst_uparams]) args in
         (* get and lift the instantiation *)
-        let ' (llargs, arg_to_sub) := nth k inst_uparams_a err_arg in
+        let ' (llargs, arg_to_sub) := nth k inst_uparams_no_rc err_arg in
         let llargs := map (lift0 (pos_sub_cxt + #|largs|)) llargs in
-        (* 0 ????? => #|llargs| ? *)
         let arg_to_sub := lift_argument (pos_sub_cxt + #|largs|) #|llargs| arg_to_sub in
         sub_uparam largs' args' llargs arg_to_sub
     | arg_is_ind largs i inst_uparams_indices =>
         let largs' := mapi_rec (fun i t => t.[up i inst_uparams]) largs pos_sub_cxt in
         (* we need to add var for new nup + new indices - old_nup *)
-        let new_indices := tRels (pos_sub_cxt + #|largs|) (nb_g_nuparams + #|g_Γargs| + #|g_largs_t|) in
+        let new_indices := tRels (pos_sub_cxt + #|largs|) (nb_g_nuparams + nb_g_args_no_rc + #|g_largs|) in
         (* nup are now indices so just need to be updated *)
         let inst_uparams_indices'  := map (fun t => t.[up (pos_sub_cxt + #|largs|) inst_uparams]) inst_uparams_indices in
         arg_is_ind largs' (i + nb_g_block) (new_indices ++ inst_uparams_indices')
@@ -500,49 +800,42 @@ Section NestedToMutualInd.
         arg_is_nested largs' ind u insta_uparams' inst_nuparams_indices'
     end.
 
-  (* Γargs |- arg *)
-  Section SpeArg.
-  Context (Γargs : list argument).
 
-
-
-  (* Definition length_nΓargs : #|nΓargs| = #|Γargs|.
-  Admitted. *)
-
-  Definition pos_specialize_argument lax nb_binders arg :
-    positive_argument nb_l_block l_uparams_b l_nuparams (map check_lax Γargs) lax nb_binders arg ->
+  Definition pos_specialize_argument Γ lax nb_binders arg :
+    positive_argument nb_l_block l_uparams_b l_nuparams (map check_lax Γ) lax nb_binders arg ->
     positive_argument nb_m_block g_uparams_b g_nuparams
-      (map check_lax (cstr_new_args ++ (mapi_rec specialize_argument Γargs nb_l_nuparams)))
-      lax nb_binders (specialize_argument (nb_l_nuparams + #|Γargs| + nb_binders) arg).
+      (map check_lax (cstr_new_args ++ (mapi_rec specialize_argument Γ nb_l_nuparams)))
+      lax nb_binders (specialize_argument (nb_l_nuparams + #|Γ| + nb_binders) arg).
   Proof.
-    (* rewrite length_nΓargs. *)
+  (* Admitted. *)
     intro pos_arg; induction pos_arg using positive_argument_rect'; cbn.
     + apply pos_arg_is_free; rewrite -> ? length_map in *.
-      apply inst_preserve_not_eq => //. solve_length.
+      apply inst_preserve_not_eq => //. cbn_length. lia.
     + rewrite <- Nat.add_assoc.
-      destruct (nth k inst_uparams_a err_arg) as [llargs arg_to_sub] eqn:H.
+      destruct (nth k inst_uparams_no_rc err_arg) as [llargs arg_to_sub] eqn:H.
       apply eq_prod in H as [Hfst Hsnd]. cbn_length.
       apply pos_sub_uparams. all: cbn_length; rewrite -> ? length_map in *.
       - apply Alli_notin_eq => //. lia.
       - apply All_notin_eq => //. lia.
       - rewrite - fapp -Hfst. symmetry.
         apply (All2_nth (fun n x => n = #|x.1|)); only 1: solve_length.
-        apply fapp_inst_uparams.
+        apply fapp_inst_uparams_no_rc.
       - eapply (Alli_map_gen_eq
-          (n := nb_cxt_sub)
-          (k := nb_l_nuparams + #|Γargs| + nb_binders + #|largs|)).
+          (n := nb_new_cxt_sub)
+          (k := nb_l_nuparams + #|Γ| + nb_binders + #|largs|)).
         * lia.
         * intros n x H. rewrite Nat.add_comm. unfold ind_sp_uparams_notin.
-          rewrite -shiftnP_add. rewrite -{1}(Nat.add_0_r (nb_l_nuparams + #|Γargs| + nb_binders + #|largs|)).
+          rewrite -shiftnP_add. rewrite -{1}(Nat.add_0_r (nb_l_nuparams + #|Γ| + nb_binders + #|largs|)).
           apply on_free_vars_lift_impl. rewrite shiftnP_add; cbn. exact H.
-        * rewrite -Hfst. apply All_nth => //. 1: rewrite size_inst_uparams; lia.
-          apply positive_inst_llargs.
+        * rewrite -Hfst. apply All_nth => //. 1: rewrite size_inst_uparams_no_rc; lia.
+          apply positive_inst_llargs_no_rc.
       - apply pos_arg_inc => //.
-        assert (positive_argument nb_g_block g_uparams_b g_nuparams (map check_lax g_Γargs) lax (nb_g_largs + #|llargs|) arg_to_sub).
-        1: { rewrite -Hfst -Hsnd. apply All_nth => //. 1: rewrite size_inst_uparams; lia.
-             destruct lax; only 2: inversion e. apply positive_true_all.
+        (* wrong args *)
+        assert (positive_argument nb_g_block g_uparams_b g_nuparams (map check_lax g_args_no_rc) lax (nb_g_largs + #|llargs|) arg_to_sub).
+        1: { rewrite -Hfst -Hsnd. apply All_nth => //. 1: rewrite size_inst_uparams_no_rc; lia.
+             destruct lax; only 2: inversion e. apply positive_true_all_no_rc.
           }
-        eapply @pos_lift_argument_eq with (Γargs1 := (map check_lax (g_Γargs ++ map arg_is_free g_largs_t))) (nb_binders := 0) (n := nb_binders + #|largs|).
+        eapply @pos_lift_argument_eq with (Γargs1 := (map check_lax (g_args_no_rc ++ map arg_is_free g_largs_no_rc))) (nb_binders := 0) (n := nb_binders + #|largs|).
         * reflexivity.
         * rewrite !map_app -!app_assoc. reflexivity.
         * lia.
@@ -566,9 +859,6 @@ Section NestedToMutualInd.
         * apply_eq p. f_equal. lia.
   Qed.
 
-  End SpeArg.
-
-
   (* The instanciation of the uniform parameters is defined in the context:
 
         g_uparams ,,, g_nuparams ,,, g_args ,,, g_largs |- inst_uparams
@@ -579,10 +869,10 @@ Section NestedToMutualInd.
 
       We then have as a new type:
 
-         (g_args ,,, g_largs), σ(l_nuparams ,,, cstr_args)
-          |- new_indices ++ σ #|l_nupar + cstr_args| cstr_indices
+         (↓↓g_args ,,, ↓g_largs), (↓σ)(l_nuparams ,,, cstr_args)
+          |- new_indices ++ (↓σ) #|l_nuparams ,,, cstr_args| cstr_indices
 
-      Note, we must also add cstr_indices as g_args ,,, g_largs), σ(l_nuparams)
+      Note, we must also add new_indices as g_args ,,, g_largs), σ(l_nuparams)
       are now indices!
   *)
 
@@ -592,7 +882,7 @@ Section NestedToMutualInd.
     cstr_name     := todo;
     cstr_args    := cstr_new_args
                     ++ mapi (fun i => specialize_argument (nb_l_nuparams + i)) ctor.(cstr_args)  ;
-    cstr_indices :=    tRels #|ctor.(cstr_args)| (#|g_Γargs| + #|g_largs_t| + #|l_nuparams|)
+    cstr_indices :=    tRels #|ctor.(cstr_args)| (#|g_args_no_rc| + #|g_largs| + #|l_nuparams|)
                     ++ map (inst (up (nb_l_nuparams + #|ctor.(cstr_args)|) inst_uparams))
                            ctor.(cstr_indices)
   |}.
@@ -614,12 +904,12 @@ Section NestedToMutualInd.
         * cbn. apply All_telescope_singleton.
           unfold mapi. rewrite -mapi_rec_add. fold specialize_argument.
           rewrite {1}Nat.add_0_r app_nil_r Nat.add_assoc.
-          apply pos_specialize_argument with (Γargs := Γ).
+          apply pos_specialize_argument with (Γ := Γ).
           assumption.
     + cbn_length. apply All_app_inv.
       - unfold tRels. apply All_rev_pointwise_map; cbn.
         intros. apply shiftnP_lt. lia.
-      - apply All_notin_eq; only 1: lia. assumption.
+      - apply All_notin_eq; tea. lia.
   Qed.
 
   Definition specialize_one_inductive_body (idecl : one_inductive_body) : one_inductive_body :=
@@ -632,14 +922,33 @@ Section NestedToMutualInd.
     ind_relevance := todo;
   |}.
 
+  Definition ind_sp_up_impl_sp_up : forall (n : nat) (x : term),
+    ind_sp_uparams_notin g_uparams_b n x ->
+    sp_uparams_notin g_uparams_b n x.
+  Proof.
+    intros n x. apply on_free_vars_impl, shiftnP_impl.
+    unfold ind_sp_uparams_notinP; cbn.
+    intros i H%andb_prop; apply H.
+  Qed.
+
   Definition pos_specialize_idecl idecl :
     positive_one_inductive_body nb_l_block l_uparams_b l_nuparams idecl ->
     positive_one_inductive_body nb_m_block g_uparams_b g_nuparams (specialize_one_inductive_body idecl).
   Proof.
     intros [Ha Hb]; split; cbn.
-    - now eapply All_map; only 1: apply pos_specialize_ctor.
+    + now eapply All_map; only 1: apply pos_specialize_ctor.
     (* one extra case if you want to prove it is not inductiv inductive *)
-    - admit.
+    + unfold new_indices. rewrite ?rev_app_distr ?map_app.
+      repeat apply Alli_app_inv; cbn_length.
+      - unfold arguments_to_context.
+        rewrite List.rev_involutive -(map_mapi _ _ vassAR) map_map /= map_id.
+        (* should be easya-ish s only keep "non rc" *)
+        admit.
+      - unfold cxt_of_terms.
+        rewrite List.rev_involutive map_map /= map_id.
+        eapply Alli_impl; only 1 : apply pos_g_largs_no_rc; cbn.
+        apply ind_sp_up_impl_sp_up.
+      - admit. (* gonna be hell *)
   Admitted.
 
 End NestedToMutualInd.
@@ -683,8 +992,9 @@ Section NestedToMutualIndb.
                                   g_uparams_b g_nuparams nargs largs mdecl.(ind_nuparams)
                                   inst_uparams) mdecl.(ind_bodies) in
             (* we need to add var for new nup + new indices i.e *)
-            let new_indices := tRels 0 (nb_g_nuparams + #|nargs| + #|largs|) in
-
+            let new_indices := tRels 0 nb_g_nuparams
+              ++ filter2 (map check_lax nargs) (tRels nb_g_nuparams #|nargs|)
+              ++ tRels (nb_g_nuparams + #|nargs|) #|largs| in
           let new_arg := arg_is_ind largs (pos_indb + nb_g_block + #|acc_indb|)
                           (new_indices ++ inst_nuparams_indices) in
           (nargs ++ [new_arg], acc_indb ++ new_indb))
@@ -698,8 +1008,8 @@ Section NestedToMutualIndb.
 
   Definition PosAcc (acc : Acc) : Type :=
       let nargs := acc.1 in let acc_indb := acc.2 in
-        All_telescope (fun Γargs => positive_argument (nb_g_block + #|acc_indb|)
-                        g_uparams_b g_nuparams (map check_lax Γargs) true 0) nargs
+        All_telescope (fun Γ => positive_argument (nb_g_block + #|acc_indb|)
+                        g_uparams_b g_nuparams (map check_lax Γ) true 0) nargs
     * (All (positive_one_inductive_body (nb_g_block + #|acc_indb|) g_uparams_b g_nuparams) acc_indb).
 
   Tactic Notation "solve_nested_to_mut" :=
@@ -725,9 +1035,10 @@ Section NestedToMutualIndb.
     + apply All_telescope_app_inv. 1: (eapply All_telescope_impl; tea; intros; apply pos_arg_inc) => //.
       apply All_telescope_singleton; rewrite app_nil_r. constructor; cbn_length => //.
       1: { rewrite -mutual_to_view_ind. lia. }
-      apply All_app_inv => //.
-      unfold tRels. apply All_rev_pointwise_map. cbn.
-      intros. apply shiftnP_lt. lia.
+      apply All_app_inv => //. repeat apply All_app_inv.
+      - apply All_rev_pointwise_map; intros; apply shiftnP_lt; lia.
+      - apply All_filter2, All_rev_pointwise_map; intros; apply shiftnP_lt; lia.
+      - apply All_rev_pointwise_map; intros; apply shiftnP_lt; lia.
     + apply All_app_inv; only 1: (eapply All_impl; tea; intros; apply pos_idecl_inc) => //.
       eapply All_map; [| apply pos_l_indb ].
       intros idecl. apply pos_specialize_idecl => //.
