pcuic/theories/Bidirectional/BDStrengthening.v
@@ -6,7 +6,10 @@ From MetaRocq.Common Require Import config.
 From MetaRocq.PCUIC Require Import PCUICAst PCUICAstUtils PCUICGlobalEnv
   PCUICTactics PCUICCumulativity
   PCUICInduction PCUICLiftSubst PCUICUnivSubst PCUICEquality PCUICUtils
-  PCUICPosition PCUICTyping PCUICSigmaCalculus PCUICOnFreeVars PCUICClosed PCUICConfluence PCUICSpine PCUICInductiveInversion PCUICParallelReductionConfluence PCUICWellScopedCumulativity PCUICClosed PCUICRenameDef PCUICInstConv PCUICClosedTyp PCUICWeakeningEnvTyp PCUICRenameTyp PCUICRenameConv PCUICGuardCondition PCUICWeakeningConv.
+  PCUICPosition PCUICTyping PCUICSigmaCalculus PCUICOnFreeVars PCUICClosed
+  PCUICConfluence PCUICSpine PCUICInductiveInversion PCUICParallelReductionConfluence
+  PCUICWellScopedCumulativity PCUICClosed PCUICRenameDef PCUICInstConv PCUICClosedTyp
+  PCUICWeakeningEnvTyp PCUICRenameTyp PCUICRenameConv PCUICGuardCondition PCUICWeakeningConv.
 
 From MetaRocq.PCUIC Require Import BDTyping BDToPCUIC BDFromPCUIC.
 
